Complete cut

theories/Cut.v
@@ -5,357 +5,385 @@ Require Import Stdlib.Program.Equality.
 
 Local Hint Rewrite @elements_env_add : order.
 
+Definition CutHyp (w : nat) :=
+  forall (φ : form), weight φ <= w -> 
+  forall (ψ : form) (Γ : env), Γ ⊢ φ -> (Γ • φ) ⊢ ψ -> Γ ⊢ ψ.
+
+Definition ImpOrForAll (φ : form) := 
+  (exists A B, φ = (Implies A B)) \/ (exists A, φ = (ForAll A)).
+
+Lemma cutM {w : nat} (IHw : CutHyp w) (θ : form) (hθ : weight θ <= w) 
+  (Γ1 Γ2 : env) (ψ : form) (d1 : Γ1 ⊢ θ) (d2 : (Γ2 • θ) ⊢ ψ) : (Γ1 ⊎ Γ2) ⊢ ψ.
+Proof.
+  intros.
+  apply (IHw θ).
+  - lia.
+  - now apply generalised_weakeningR.
+  - peapply (generalised_weakeningL _ Γ1 _ d2).
+Qed.
+        
+Lemma hshape (σ : nat -> term) (θ : form) (hθ : ImpOrForAll θ) :
+  ImpOrForAll (subst_form σ θ).
+Proof.
+  destruct hθ.
+  - destruct H as [A H]; destruct H as [B Heq]; subst; simpl; left.
+    exists (subst_form σ A); exists (subst_form σ B); easy.
+  - destruct H as [A Heq]; subst; right.
+    exists (subst_form (up σ) A); easy.
+Qed.
+
+Lemma cut_principal (w : nat) (IHw : CutHyp w) 
+  (Δ : env) (θ : form) (h : Δ ⊢ θ) :
+  forall (φ : form) (Γ Γ' : env), 
+    Δ = (Γ' • φ) -> 
+    weight φ <= w + 1 -> 
+    ImpOrForAll φ -> 
+    Γ ⊢ φ -> 
+    (Γ ⊎ Γ') ⊢ θ.
+Proof.
+  induction h; intros φ0 Γ0 Γ' HeqΓ Hw HImp Hp.
+  - destruct (decide (φ0 = (Atom i xs))) as [Heq | Hneq]. 
+    + subst; exfalso; destruct HImp as [[A [B Heq]] | [A Heq']]; discriminate.
+    + assert (Hin : Atom i xs ∈ Γ') by multiset_solver.
+      apply generalised_weakeningL; exhibit Hin 0; auto with proof.
+  - case (decide (Bot = φ0)) as [Heq | Hneq].
+    + subst; exfalso; destruct HImp as [[A [B Heq]] | [A Heq']]; discriminate.
+    + assert (Hin : ⊥ ∈ Γ') by multiset_solver.
+      apply generalised_weakeningL; exhibit Hin 0; auto with proof.
+  - apply AndR; [apply IHh1 with (φ := φ0); auto |
+                  apply IHh2 with (φ := φ0); auto ].
+  - case (decide ((And φ ψ) = φ0)) as [Heq | Hneq].
+    + subst; exfalso; destruct HImp as [[A [B Heq]] | [A Heq']]; discriminate.
+    + assert (Hin : (And φ ψ) ∈ Γ') by multiset_solver.
+      replace (Γ0 ⊎ Γ') with (Γ0 ⊎ (Γ ∖ {[φ0]}) • (φ ∧ ψ)) by multiset_solver.
+      apply AndL.
+      replace (Γ0 ⊎  (Γ) ∖ {[φ0]} • φ • ψ) with
+                                                                                (Γ0 ⊎ (Γ ∖ {[φ0]} • φ • ψ)) by ms.
+      apply (IHh φ0 Γ0); multiset_solver; auto.
+  - apply OrR1. apply IHh with (φ := φ0); auto.
+  - apply OrR2. apply IHh with (φ := φ0); auto.
+  - case (decide ((Or φ ψ) = φ0)) as [Heq | Hneq].
+    + subst; exfalso; destruct HImp as [[A [B Heq]] | [A Heq']]; discriminate.
+    + assert (Hin : (Or φ ψ) ∈ Γ') by multiset_solver.
+      replace (Γ0 ⊎ Γ') with (Γ0 ⊎ (Γ ∖ {[φ0]}) • (φ ∨  ψ)) by multiset_solver.
+      peapply OrL.
+      replace (Γ0 ⊎  (Γ) ∖ {[φ0]} • φ) with                                           (Γ0 ⊎ (Γ ∖ {[φ0]} • φ)) by ms.
+      apply IHh1 with (φ := φ0); multiset_solver; auto.
+      replace (Γ0 ⊎  (Γ) ∖ {[φ0]} • ψ) with                                           (Γ0 ⊎ (Γ ∖ {[φ0]} • ψ)) by ms.
+      apply IHh2 with (φ := φ0); multiset_solver; auto.
+  - apply ImpR.
+    replace  (Γ0 ⊎ Γ' • φ) with  (Γ0 ⊎ (Γ' • φ)) by ms.
+    apply IHh with (φ := φ0); ms.
+  - destruct (decide ((Implies (Atom i xs) φ) = φ0)).
+    + assert (HeqΓ' : (Γ • (Atom i xs)) = Γ') by ms.
+      assert (Hin: (Atom i xs) ∈ (Γ0 ⊎ Γ')) by ms.
+      exhibit Hin 0.
+      apply contraction.
+      backward.
+      rewrite env_add_remove.
+      replace  (Γ0 ⊎ Γ' • Atom i xs) with ( (Γ0 • Atom i xs) ⊎ Γ').
+      subst.
+      apply (cutM IHw φ).
+      simpl in Hw. lia.
+      apply ImpR_rev; easy.
+      easy.
+      ms.
+    + case (decide ((Atom i xs) = φ0)) as [Heq | Hneq].
+      * subst; exfalso; destruct HImp as [[A [B Heq]] | [A Heq']]; discriminate.
+      * assert (Hin'' : (Implies (Atom i xs) φ) ∈ Γ') by multiset_solver.
+        assert (Hin' : (Implies (Atom i xs) φ) ∈ (Γ0 ⊎ Γ')) by multiset_solver.
+        exhibit Hin' 0.
+        assert (Hin : (Atom i xs) ∈ (Γ0 ⊎ Γ') ∖ {[+ (Implies (Atom i xs) φ) +]}) by multiset_solver.
+        
+        exhibit Hin 1.
+        apply ImpL0.
+        exch 0.
+        backward.
+        rewrite env_add_remove.
+        replace ((Γ0 ⊎ Γ') ∖ {[+ Atom i xs → φ +]} • φ) with  (Γ0 ⊎  (Γ' ∖ {[+ Atom i xs → φ +]} • φ)) by multiset_solver.
+        
+        apply (IHh φ0).
+        multiset_solver.
+        lia.
+        easy.
+        easy.
+  - case (decide ((Implies (φ1 ∧ φ2) φ3) = φ0)) as [Heq | Hneq].
+    + assert (Γ = Γ') by ms.
+      subst.
+      apply (IHw (φ1 → φ2 → φ3)). simpl in *; lia.
+      apply ImpR, ImpR, AndL_rev.
+      peapply ImpR_rev.
+      apply generalised_weakeningR.
+      easy.
+      replace ( (Γ0 ⊎ Γ' • (φ1 → φ2 → φ3)) ) with (Γ0 ⊎ (Γ' • (φ1 → φ2 → φ3))) by ms.
+      apply generalised_weakeningL.
+      easy.
+    + assert (Hin: (Implies (φ1 ∧ φ2) φ3) ∈ Γ') by multiset_solver.
+      replace (Γ0 ⊎ Γ') with
+        ((Γ0 ⊎ (Γ' ∖ {[φ1 ∧ φ2 → φ3]})) • (φ1 ∧ φ2 → φ3)) by multiset_solver.
+      apply ImpLAnd.
+      peapply (IHh φ0 Γ0 ((Γ'∖ {[φ1 ∧ φ2 → φ3]}) • (φ1 → φ2 → φ3))).
+      multiset_solver.
+      lia.
+      easy.
+      easy.      
+  - destruct (decide ((φ1 ∨ φ2 → φ3) = φ0)) as [Heq | Hneq].
+    + assert (Γ = Γ') by ms. subst.
+      clear HeqΓ.
+      apply ImpR_rev in Hp.
+      apply OrL_rev in Hp.
+      destruct Hp.
+      apply (IHw (φ1 → φ3)).      
+      simpl in *; lia.
+      apply generalised_weakeningR.
+      apply ImpR; easy.
+      apply (IHw (φ2 → φ3)).
+      simpl in *; lia.
+      replace ( (Γ0 ⊎ Γ') • (φ1 → φ3) ) with (Γ' ⊎ (Γ0 • (φ1 → φ3))) by ms.
+      apply generalised_weakeningL.
+      apply ImpR. exch 0.
+      auto with proof.
+      
+      replace ( (Γ0 ⊎ Γ') • (φ1 → φ3) • (φ2 → φ3) )
+        with (Γ0 ⊎ (Γ' • (φ1 → φ3) • (φ2 → φ3) )) by ms.
+      apply generalised_weakeningL.
+      easy.
+    + assert (Hin : (φ1 ∨ φ2 → φ3) ∈ Γ') by multiset_solver.      
+      peapply (ImpLOr (Γ0 ⊎ (Γ' ∖ {[φ1 ∨ φ2 → φ3]})) φ1 φ2 φ3).      
+      peapply (IHh φ0 Γ0 (Γ' ∖ {[φ1 ∨ φ2 → φ3]} • (φ1 → φ3) • (φ2 → φ3))).
+      multiset_solver.
+      lia.
+      easy.
+      easy.
+      multiset_solver.
+  - destruct (decide ((Implies (Implies φ1 φ2) φ3) = φ0)) as [Heq | Hneq].
+    + assert (Γ = Γ') by ms.
+      subst.
+      clear HeqΓ.
+      apply ImpR_rev in Hp.
+      apply (cutM IHw φ3) with (Γ2 := Γ') (ψ := ψ) in Hp as Hp2; [ | simpl in *; lia | easy].
+      replace ((Γ0 • (φ1 → φ2)) ⊎ Γ') with ((Γ0 ⊎ Γ')• (φ1 → φ2)) in Hp2 by ms.
+      apply (IHw (φ1 → φ2)); [ simpl in *; lia | | easy ].
+      apply ImpR.
+      apply (IHw (φ2 → φ3)); [ simpl in *; lia | | 
+      replace  (Γ0 ⊎ Γ' • φ1 • (φ2 → φ3)) with  (Γ0 ⊎ (Γ' • φ1 • (φ2 → φ3))) by ms; apply generalised_weakeningL; easy].
+      apply ImpR.
+      apply (IHw (φ1 → φ2)); [ simpl in *; lia | apply ImpR; exch 0; apply generalised_axiom |].
+      replace (Γ0 ⊎ Γ' • φ1 • φ2 • (φ1 → φ2))
+           with ((Γ0 • (φ1 → φ2)) ⊎ (Γ' • φ1 • φ2)) by ms.
+      apply generalised_weakeningR; easy.
+    + assert (Hin : ((φ1 → φ2) → φ3) ∈ Γ') by multiset_solver.      
+      peapply (ImpLImp (Γ0 ⊎ (Γ' ∖ {[(φ1 → φ2) → φ3]})) φ1 φ2 φ3).
+      peapply (IHh1 φ0 Γ0 (Γ' ∖ {[(φ1 → φ2) → φ3]}  • φ1 • (φ2 → φ3) )).
+      multiset_solver.
+      lia.
+      easy.
+      easy.
+      peapply (IHh2 φ0 Γ0 (Γ' ∖ {[(φ1 → φ2) → φ3]}  • φ3  )).
+      multiset_solver.
+      lia.
+      easy.
+      easy.
+      multiset_solver.
+  - apply ForAllR.
+    replace ( gmultiset_map (subst_form S') (Γ0 ⊎ Γ')) with
+      ((gmultiset_map (subst_form S') Γ0) ⊎ (gmultiset_map (subst_form S') Γ'))by (symmetry; apply gmultiset_map_disj_union).
+    apply IHh with (φ := (subst_form S' φ0)).
+    subst.
+    apply  gmultiset_map_distr_disj_union_singleton.
+    rewrite weight_subst_f.
+    lia.
+    apply hshape. easy.
+    apply relabelling_lemma.
+    easy.
+  - destruct (decide ((ForAll φ) = φ0)) as [Heq | Hneq].
+    + assert (Γ = Γ') by ms.
+      subst.
+
+      assert (Hp1 : Γ0 ⊢ (subst_form (bind_var t) φ)).
+      apply ForAllR_rev_specialised.
+      easy.
+      assert (Hp2 : Γ0 ⊎ Γ' ⊢ (subst_form (bind_var t) φ)).
+      apply generalised_weakeningR.
+      easy.
+
+      apply generalised_contraction.
+      replace (Γ0 ⊎ Γ0 ⊎ Γ') with (Γ0 ⊎ (Γ0 ⊎ Γ')) by ms.
+      apply (cutM IHw (subst_form (bind_var t) φ))
+        with (Γ2 := (Γ0 ⊎ Γ')).
+      rewrite weight_subst_f; simpl in Hw; lia.
+      easy.
+
+      replace  (Γ0 ⊎ Γ' • φ 〔 bind_var t 〕) with
+        (Γ0 ⊎ (Γ' • φ 〔 bind_var t 〕)) by ms.
+
+      apply (IHh (ForAll φ)).
+      ms.
+      easy.
+      easy.
+      easy.
+    + assert (Hin: ForAll φ ∈ Γ') by multiset_solver.
+      peapply (ForAllL (Γ0 ⊎ (Γ' ∖ {[ ForAll φ ]})) φ ψ t).
+      peapply (IHh φ0 Γ0
+                 (Γ' ∖ {[ForAll φ]} • (ForAll φ) • φ 〔 bind_var t 〕)
+              ).
+      multiset_solver.
+      easy.
+      easy.
+      easy.
+      multiset_solver.
+  - apply ExistsR with (t := t).
+    apply IHh with (φ := φ0); easy.
+  - case (decide ((Exists φ) = φ0)) as [Heq | Hneq].
+    + subst; exfalso; destruct HImp as [[A [B Heq]] | [A Heq']]; discriminate.
+    + assert (Hin: (Exists φ) ∈ Γ') by multiset_solver.
+      peapply (ExistsL (
+                   Γ0 ⊎ (Γ' ∖ {[Exists φ]})
+                 ) φ).
+      assert (HeqΓMap :
+          ((gmultiset_map (subst_form S') Γ0) ⊎ (gmultiset_map (subst_form S') (Γ' ∖ {[Exists φ]}))) = 
+        (gmultiset_map (subst_form S') (Γ0 ⊎ Γ' ∖ {[Exists φ]}))
+             ) by (apply symmetry, gmultiset_map_disj_union).
+      replace (gmultiset_map (subst_form S') (Γ0 ⊎ Γ' ∖ {[Exists φ]}) • φ) with
+        ((gmultiset_map (subst_form S') Γ0) ⊎
+           ((gmultiset_map (subst_form S') (Γ' ∖ {[Exists φ]})) • φ)) by ms.
+      pose (gmultiset_map_distr_disj_union_singleton (subst_form S')) as H1.
+      pose (gmultiset_map_eq (subst_form S')) as H2.
+     
+      apply (IHh (subst_form S' φ0)); try easy.
+      * unfold_leibniz.
+        rewrite env_add_comm.
+        apply equiv_disj_union_compat_r.
+        rewrite <- H1.
+        apply H2.
+        multiset_solver.
+      * rewrite weight_subst_f; lia.
+      * apply hshape; easy.
+      * apply relabelling_lemma; easy.
+      * multiset_solver.
+  - destruct (decide (((ForAll φ1) → φ2) = φ0)) as [Heq | Hneq].
+    + assert (Γ' = Γ) by ms.
+      subst.
+      clear HeqΓ.
+      apply ImpR_rev in Hp as Hp'.
+      
+      assert (Hp2: (Γ0 ⊎ Γ) • (ForAll φ1) ⊢ ψ).
+      replace (Γ0 ⊎ Γ • (ForAll φ1)) with ((Γ0 • (ForAll φ1)) ⊎ Γ) by ms.
+      apply (cutM IHw φ2); [ simpl in *; lia | easy | easy ].
+      apply (IHh1 (Implies (ForAll φ1) φ2) Γ0 Γ) in Hp as Hp''; try easy.
+      replace (Γ0 ⊎ Γ) with ((Γ0 ⊎ Γ) ⊎ ∅) by ms.
+      apply generalised_contraction with (Γ := ∅) (Γ' := (Γ0 ⊎ Γ)). 
+      replace ( Γ0 ⊎ Γ ⊎ (Γ0 ⊎ Γ) ⊎ ∅) with ((Γ0 ⊎ Γ) ⊎ (Γ0 ⊎ Γ)) by ms.
+      apply (cutM IHw (ForAll φ1)); [ simpl in *; lia | easy | easy].
+    + assert (Hin : ((ForAll φ1) → φ2) ∈ Γ' ) by multiset_solver.
+      peapply (ImpLForAll (Γ0 ⊎ (Γ' ∖ {[ (ForAll φ1) → φ2 ]})) φ1 φ2).
+      peapply (IHh1 φ0 Γ0 Γ').
+      multiset_solver.
+      simpl in Hw; lia.
+      easy.
+      easy.
+      multiset_solver.
+      peapply (IHh2 φ0 Γ0 ((Γ' ∖ {[ (ForAll φ1) → φ2 ]}) • φ2)).
+      multiset_solver.
+      lia.
+      easy.
+      easy.
+      multiset_solver.      
+  - destruct (decide ((Implies (Exists φ1) φ2) = φ0)) as [Heq | Hneq].
+    + assert (Γ' = Γ) by ms.
+      subst.
+      clear HeqΓ.
+      apply ImpR_rev in Hp as Hp'.
+      apply ExistsL_rev in Hp'.
+      
+      apply (IHh (ForAll (Implies φ1 (subst_form S' φ2)))); [
+          easy
+        | simpl in *; rewrite weight_subst_f; lia
+        | right; exists (Implies φ1 (subst_form S' φ2)); easy |].
+      apply ForAllR.
+      apply ImpR.
+      easy.
+    + assert (Hin: ((Exists φ1) → φ2) ∈ Γ') by multiset_solver.
+      peapply (ImpLExists (Γ0 ⊎ (Γ' ∖ {[ (Exists φ1) → φ2 ]})) φ1 φ2).
+
+      peapply (IHh φ0 Γ0 (Γ' ∖ {[ (Exists φ1) → φ2 ]} • (ForAll (φ1 → φ2〔 S' 〕 ) ))).
+      multiset_solver.
+      lia.
+      easy.
+      easy.
+      multiset_solver.
+Qed.
+      
+Lemma cut_principal_add (w : nat) (IHw : CutHyp w) (φ : form) (Γ : env)
+  (hφ : weight φ <= w + 1) (hk : ImpOrForAll φ) (hd : Γ ⊢ φ) (ψ : form)
+  (h2 : (Γ • φ) ⊢ ψ) : Γ ⊢ ψ.
+Proof.
+  replace Γ with (Γ ⊎ ∅) by ms.
+  apply generalised_contraction.
+  replace ((Γ ⊎ Γ) ⊎ ∅) with (Γ ⊎ Γ).
+  apply cut_principal with  (φ := φ) (Δ :=  (Γ • φ)) (w := w); try easy.
+  - ms.
+Qed.
+
 (* From "A New Calculus for Intuitionistic Strong Löb Logic" *)
 Theorem additive_cut  Γ φ ψ :
   Γ ⊢ φ  -> Γ • φ ⊢ ψ ->
   Γ ⊢ ψ.
 Proof.
-  (* Get induction on weight *)
-remember (weight φ) as w. assert(Hw : weight φ ≤ w) by lia. clear Heqw.
-revert φ Hw ψ Γ.
-induction w; intros φ Hw; [pose (weight_pos φ); lia|].
-intros ψ Γ.
+  remember (weight φ) as w. assert(Hw : weight φ ≤ w) by lia. clear Heqw.
+  revert φ Hw ψ Γ.
+  induction w; intros φ Hw; [pose (weight_pos φ); lia|].
 
-(*remember (height HPφ + height HPψ) as h.
-assert(Hleh : height HPφ + height HPψ ≤ h) by lia. clear Heqh.
-revert Γ φ ψ HPφ HPψ Hw Hleh.
-induction h; intros; [ pose (height_0 HPφ); lia |]. *)
-
-remember (Γ, ψ) as pe.
-replace Γ with pe.1 by now subst.
-replace ψ with pe.2 by now subst. clear Heqpe Γ ψ. revert pe φ Hw.
-refine  (@well_founded_induction _ _ wf_pointed_env_ms_order _ _).
-intros (Γ &ψ). simpl. intro IHW'. assert (IHW := fun Γ0 => fun ψ0 => IHW' (Γ0, ψ0)).
-simpl in IHW. clear IHW'. intros φ Hw HPφ HPψ.
-Ltac otac Heq := subst; repeat rewrite env_replace in Heq by trivial; repeat rewrite env_add_remove by trivial; order_tac; rewrite Heq; order_tac.
-                                                       
-destruct HPφ; simpl in Hw.
+  intros ψ Γ HPφ HPψ.
+  revert ψ HPψ.
+  induction HPφ; simpl in Hw; intros.
 - now apply contraction.
 - apply ExFalso.
 - apply AndL_rev in HPψ. do 2 apply IHw in HPψ; trivial; try lia; apply weakening; assumption.
-- apply AndL. apply IHW with (φ := θ); auto with proof. order_tac.
-- apply OrL_rev in HPψ; apply (IHw φ); [lia| |]; tauto.
-- apply OrL_rev in HPψ; apply (IHw ψ0); [lia| |]; tauto.
-- apply OrL; apply IHW with (φ := θ); auto with proof.
-  + otac Heq.
-  + exch 0. eapply (OrL_rev _ φ ψ0). exch 0. exact HPψ.
-  + order_tac.
-  + exch 0. eapply (OrL_rev _ φ ψ0). exch 0. exact HPψ.
-- (* (V) *) (* hard:  *)
-  (* START *)
-  remember (Γ • (φ → ψ0)) as Γ' eqn:HH.
-  assert (Heq: Γ ≡ Γ' ∖ {[ φ → ψ0]}) by ms.
-  assert (Hin : (φ → ψ0) ∈ Γ')by ms.
-  rw Heq 0. destruct HPψ.
-  + forward. auto with proof.
-  + forward. auto with proof.
-  + apply AndR.
-     * rw (symmetry Heq) 0. apply IHW with (φ := (φ → ψ0)).
-       -- order_tac.
-       -- simpl. lia.
-       -- now apply ImpR.
-       -- peapply HPψ1.
-     * rw (symmetry Heq) 0. apply IHW with (φ := (φ → ψ0)).
-       -- order_tac.
-       -- simpl. lia.
-       -- apply ImpR. peapply HPφ.
-       -- peapply HPψ2.
-  + forward. apply AndL. apply IHW with (φ := (φ → ψ0)).
-    * unfold pointed_env_ms_order. otac Heq.
-    * simpl. lia.
-    * apply AndL_rev. backward. rw (symmetry Heq) 0. apply ImpR, HPφ.
-    * backward. peapply HPψ.
-  + apply OrR1, IHW with (φ := (φ → ψ0)).
-    * rewrite HH, env_add_remove. order_tac.
-    * simpl. lia.
-    * rw (symmetry Heq) 0. apply ImpR, HPφ.
-    * peapply HPψ.
-  + apply OrR2, IHW with (φ := (φ → ψ0)).
-    * rewrite HH, env_add_remove. order_tac.
-    * simpl. lia.
-    * rw (symmetry Heq) 0. apply ImpR, HPφ.
-    * peapply HPψ.
-  + forward. apply ImpR in HPφ.
-       assert(Hin' : (φ0 ∨ ψ) ∈ ((Γ0 • φ0 ∨ ψ) ∖ {[φ→ ψ0]}))
-            by (apply in_difference; [discriminate|ms]).
-       assert(HPφ' : (((Γ0 • φ0 ∨ ψ) ∖ {[φ→ ψ0]}) ∖ {[φ0 ∨ ψ]} • φ0 ∨ ψ) ⊢ (φ → ψ0))
-            by (rw (symmetry (difference_singleton _ (φ0 ∨ψ) Hin')) 0; peapply HPφ).
-       assert (HP := (OrL_rev  _ φ0 ψ (φ → ψ0) HPφ')).
-       apply OrL.
-      * apply IHW with (φ := (φ → ψ0)).
-        -- rewrite env_replace in Heq by trivial. order_tac. rewrite Heq. order_tac.
-        -- simpl. lia.
-        -- peapply HP.1.
-        -- exch 0. rw (symmetry (difference_singleton _ _ Hin0)) 1. exact HPψ1.
-      * apply IHW with (φ := (φ → ψ0)).
-        -- rewrite env_replace in Heq by trivial. order_tac. rewrite Heq. order_tac.
-        -- simpl. lia.
-        -- peapply HP.2.
-        -- exch 0. rw (symmetry (difference_singleton _ _ Hin0)) 1. exact HPψ2.
-  + rw (symmetry Heq) 0. apply ImpR, IHW with (φ := (φ → ψ0)).
-    -- order_tac.
-    -- simpl. lia.
-    -- apply weakening, ImpR,  HPφ.
-    -- exch 0.  rewrite <- HH. exact HPψ.
-  + case (decide ((Atom i xs → φ0) = (φ → ψ0))).
-    * intro Heq'; dependent destruction Heq'.
-      replace ((Γ0 • Atom i xs • (Atom i xs → ψ0)) ∖ {[Atom i xs → ψ0]}) with (Γ0 • Atom i xs) by ms.
-      apply (IHw ψ0).
-      -- lia.
-      -- apply contraction. peapply HPφ.
-      -- assumption.
-    * intro Hneq. do 2 forward. exch 0. apply ImpL0, IHW with (φ := (φ → ψ0)).
-      -- repeat rewrite env_replace in Heq by trivial. order_tac. rewrite Heq. order_tac.
-      -- simpl. lia.
-      -- apply ImpL0_rev. exch 0. do 2 backward.
-            rw (symmetry Heq) 0. apply ImpR, HPφ.
-        -- exch 0; exch 1. rw (symmetry (difference_singleton _ _ Hin1)) 2. exact HPψ.
-  + case (decide (((φ1 ∧ φ2) → φ3)= (φ → ψ0))).
-      * intro Heq'; dependent destruction Heq'. rw (symmetry Heq) 0.
-         apply (IHw (φ1 → φ2 → ψ0)).
-        -- simpl in *. lia.
-        -- apply ImpR, ImpR, AndL_rev, HPφ.
-        -- peapply HPψ.
-      * intro Hneq. forward. apply ImpLAnd, IHW with (φ := (φ → ψ0)).
-        -- rewrite env_replace in Heq by trivial. order_tac. rewrite Heq. order_tac.
-        -- simpl. lia.
-        -- apply ImpLAnd_rev. backward. rw (symmetry Heq) 0. apply ImpR, HPφ.
-        -- exch 0. rw (symmetry (difference_singleton _ _ Hin0)) 1. exact HPψ.
-  + case (decide (((φ1 ∨ φ2) → φ3)= (φ → ψ0))).
-      * intro Heq'; dependent destruction Heq'. rw (symmetry Heq) 0. apply OrL_rev in HPφ.
-         apply (IHw (φ1 → ψ0)).
-        -- simpl in *. lia.
-        -- apply (IHw (φ2 → ψ0)).
-           ++ simpl in *; lia.
-           ++ apply ImpR, HPφ.
-           ++ apply weakening, ImpR, HPφ.
-        -- apply (IHw (φ2 → ψ0)).
-           ++ simpl in *; lia.
-           ++ apply weakening, ImpR, HPφ.
-           ++ peapply HPψ.
-      * intro Hneq. forward. apply ImpLOr, IHW with (φ := (φ → ψ0)).
-        -- rewrite env_replace in Heq by trivial. order_tac. rewrite Heq. order_tac.
-        -- simpl. lia.
-        -- apply ImpLOr_rev. backward. rw (symmetry Heq) 0. apply ImpR, HPφ.
-        -- exch 0. exch 1. rw (symmetry (difference_singleton _ _ Hin0)) 2. exact HPψ.
-  + case (decide (((φ1 → φ2) → φ3) = (φ → ψ0))).
-    * intro Heq'. dependent destruction Heq'. rw (symmetry Heq) 0. apply (IHw ψ0).
-      -- lia.
-      -- apply (IHw(φ1 → φ2)).
-        ++ lia.
-        ++ apply (IHw (φ2 → ψ0)).
-            ** simpl in *. lia.
-            ** apply ImpR.
-               apply (IHw (φ1 → φ2)).
-               --- lia.
-               --- apply ImpR. exch 0. apply generalised_axiom.
-               --- exch 0. apply weakening. peapply HPφ.
-            ** apply ImpR. exch 0. peapply HPψ1.
-        ++ exact HPφ.
-    -- peapply HPψ2.
-   *  (* (V-d) *)
-       intro Hneq. forward. apply ImpLImp.
-      -- apply IHW with (φ := (φ → ψ0)).
-         ++ (* otac Heq. *)
-            rewrite env_replace in Heq by trivial.
-            order_tac.
-            rewrite Heq.
-            order_tac.
-         ++ simpl. lia.
-        ++ apply contraction. apply ImpLImp_dup. backward. rw (symmetry Heq) 0.
-                apply ImpR, HPφ.
-        ++ exch 0. apply ImpR_rev. exch 0. rw (symmetry (difference_singleton _ _ Hin0)) 1. apply ImpR.
-                exact HPψ1.
-      -- apply IHW with (φ := (φ → ψ0)).
-         ++ otac Heq.
-         ++ simpl. lia.
-         ++ apply ImpLImp_prev with (φ1 := φ1) (φ2 := φ2).
-            backward.
-            rw (symmetry Heq) 0.
-            apply ImpR, HPφ.
-        ++ exch 0. rw (symmetry (difference_singleton _ _ Hin0)) 1. exact HPψ2.
-  + (* QUANTIFIER CASE *)
-    apply ForAllR. replace (Γ0 ∖ {[φ → ψ0]}) with (Γ) by (unfold_leibniz; exact Heq).
-    apply IHW with (φ := (subst_form S' (φ → ψ0))).
-    -- order_tac.
-       unfold env_order, ltof.
-       rewrite !env_weight_add.
-       rewrite !env_weight_elements_subst.
-       assert (weight φ0 < weight (ForAll φ0)) as Hlt1 by (simpl; lia).
-       apply pow5_a_lt_b in Hlt1.
-       lia.
-    -- simpl.
-       pose (weight_subst_S φ) as H1.
-       pose (weight_subst_S ψ0) as H2.
-       simpl in H1, H2.
-       lia.
-    -- simpl. apply ImpR. backward_map.
-       apply relabelling_lemma with (f := S') in HPφ.
-       exact HPφ.
-       apply (inj_upN_S 0).
-    -- backward_map.
-       rewrite <- HH.
-       exact HPψ.
-  + (* TODO Currently trying to do a proof  by induction on the height of the premise *)
-    forward.
-    apply ForAllL with (t := t).
-    apply IHW with (φ := (φ → ψ0)).
-    -- rewrite env_replace in Heq by trivial.
-       order_tac.
-       rewrite Heq.
-       order_tac.
-      order_tac.
-       admit.  (* Definitely false *)
-    -- simpl. lia.
-    -- exch 0. backward. rw (symmetry Heq) 1. apply ImpR. exch 0. apply weakening. exact HPφ.
-    -- backward. rewrite env_add_remove. assumption.
-  + rw (symmetry Heq) 0. apply ExistsR with (t := t), IHW with (φ := (φ → ψ0)).
-    -- assert ( (subst_form (bind_var t) φ0) ≺f (Exists φ0) ) as H1.
-       unfold form_order.
-       pose (weight_subst_f (bind_var t)) as H2.
-       simpl in H2.
-       simpl.
-       rewrite H2.
-       lia.
-       order_tac.
-    -- simpl. lia.
-    -- apply ImpR. exact HPφ.
-    -- rw (Heq) 1. backward. rewrite env_add_remove. exact HPψ.
-  + forward. apply ExistsL. apply IHW with (φ := ((subst_form S' (φ → ψ0)))).
-    -- otac Heq.
-       unfold env_order, ltof.
-       rewrite !env_weight_add.
-       rewrite !env_weight_elements_subst.
-       pose (weight_subst_S ψ) as Hw1.
-       simpl in Hw1.
-       rewrite Hw1.
-       assert (weight φ0 < weight (Exists φ0)) as Hlt1 by (simpl; lia).
-       apply pow5_a_lt_b in Hlt1.
-       lia.
-    -- pose (weight_subst_S (φ → ψ0)) as H1.
-       simpl. simpl in H1.
-       rewrite H1.
-       lia.
-    -- simpl. 
-       apply ImpR.
-       exch 0.
-       backward_map.
-       apply ExistsL_rev.
-       backward.
-       rw (symmetry Heq) 1.
-       exact HPφ.
-    -- exch 0. backward_map.
-       backward2.
-       rewrite env_add_remove.
-       exact HPψ.
-  + case (decide (((ForAll φ1) → φ2) = (φ → ψ0))).
-    * intro Heq'. dependent destruction Heq'. rw (symmetry Heq) 0.
-      apply (IHw(  ψ0 )  ).
-      -- lia.
-      -- apply (IHw( ForAll φ1 )).
-         ++ lia.
-         ++ apply IHW with (φ := (ForAll φ1) → ψ0).
-            ** order_tac. admit. (* Definitely false *)
-            ** simpl.
-               simpl in Hw.
-               lia.
-            ** apply ImpR. exact HPφ.
-            ** rewrite <- HH. exact HPψ1.
-         ++ exact HPφ.
-      -- rw (Heq) 1. rewrite env_add_remove. exact HPψ2.
-    * intros.
-      apply IHW with (φ := (φ → ψ0)).
-      -- order_tac. admit. (* Definitely false *)
-      -- simpl. lia.
-      -- rw (symmetry Heq) 0. apply ImpR. assumption.
-      -- forward. exch 0. backward. rewrite env_add_remove.
-         apply ImpLForAll; assumption.
-  + case (decide (((Exists φ1) → φ2) = (φ → ψ0))).
-    * intro Heq'. dependent destruction Heq'. rw (symmetry Heq) 0.
-      apply (IHw( ForAll (φ1 → (subst_form S' ψ0)) )  ).   
-      -- simpl. simpl in Hw.
-         pose (weight_subst_S ψ0) as H1.
-         simpl in H1.
-         lia.
-      -- apply ForAllR, ImpR, ExistsL_rev, HPφ.
-      -- peapply HPψ.
-    * intros. forward. apply ImpLExists. apply IHW with (φ := φ → ψ0).
-      -- assert ( (ForAll (φ1 → φ2 〔 S' 〕)) ≺f  ((Exists φ1) → φ2) ).
-         unfold form_order.
-         simpl.
-         pose (weight_subst_S φ2) as H1.
-         simpl in H1.
-         rewrite H1.
-         lia.
-         otac Heq.
-      -- simpl. lia.
-      -- apply ImpLExists_rev. backward.
-         rw (symmetry Heq) 0.
-         apply ImpR, HPφ.
-      -- exch 0. apply contraction.  apply ImpLExists_rev. backward.
-         rw (symmetry Heq) 2.
-         rewrite <- HH.
-         exch 0.
-         apply weakening.
-         exact HPψ.
-- apply ImpL0. eapply IHW; eauto.
-  + otac Heq.
-  + exch 0. exch 1.  apply ImpL0_rev. exch 1. exch 0. exact HPψ.
-- apply ImpLAnd. eapply IHW; eauto.
-  + otac Heq.
-  + exch 0. apply ImpLAnd_rev. exch 0. exact HPψ.
-- apply ImpLOr. eapply IHW; eauto.
-  + order_tac.
-  + exch 0. exch 1. apply ImpLOr_rev. exch 0. exact HPψ.
+- apply AndL. apply IHHPφ; auto with proof.
+- apply OrL_rev in HPψ. apply IHHPφ. lia. destruct HPψ; easy.
+- apply OrL_rev in HPψ; apply IHHPφ. lia. destruct HPψ; easy.
+- apply OrL; [ apply IHHPφ1; auto | apply IHHPφ2; auto ].
+  + exch 0. eapply (OrL_rev _ φ ψ). exch 0. exact HPψ.
+  + exch 0. eapply (OrL_rev _ φ ψ). exch 0. exact HPψ.
+- apply cut_principal_add with (w := w) (φ := (Implies φ ψ));
+    try easy; simpl in *; try lia.
+  left.
+  exists φ, ψ. easy.
+  apply ImpR.
+  easy.
+- apply ImpL0. eapply IHHPφ; eauto.
+  exch 0; exch 1; apply (ImpL0_rev (Γ • ψ) i xs φ ψ0).
+  exch 1. exch 0; easy.
+- apply ImpLAnd. eapply IHHPφ; eauto.
+  exch 0. apply ImpLAnd_rev. exch 0. exact HPψ.
+- apply ImpLOr. eapply IHHPφ; eauto.
+  exch 0. exch 1. apply ImpLOr_rev. exch 0. exact HPψ.
 - apply ImpLImp; [assumption|].
-  apply IHW with (φ := ψ0).
-  + otac Heq.
-  + lia.
-  + assumption.
-  + exch 0. eapply ImpLImp_prev. exch 0. exact HPψ.
-- (* Copy of (V) but with ForAll *) admit.
-- apply ForAllL with (t := t). eapply IHW; eauto.
-  + order_tac.
-    admit. (* Definitely false *)
-  + exch 0. exch 1. apply ForAllL_rev. exch 0. exact HPψ.
-- (*Copy of (V) but with Exists *) admit.
-- apply ExistsL. apply IHW with (φ := subst_form S' (ψ0)).
-  + order_tac.
-    unfold env_order, ltof.
-    rewrite !env_weight_add.
-    rewrite !env_weight_elements_subst.
-    pose (weight_subst_S ψ) as Hw1.
-    simpl in Hw1.
-    rewrite Hw1.
-    assert (weight φ < weight (Exists φ)) as Hlt1 by (simpl; lia).
-    apply pow5_a_lt_b in Hlt1.
-    lia.
-  + pose (weight_subst_S ψ0) as H1.
-    simpl in H1.
-    lia.
-  + exact HPφ.
-  + exch 0. backward_map. apply ExistsL_rev. exch 0. exact HPψ.
-- apply ImpLForAll.
-  + apply IHW with (φ := ψ0).
-    * order_tac.
-      admit. (* Definately false *)
-    * lia.
-    * apply ImpLForAll; assumption.
-    * apply weakening; assumption.
-  + eapply IHW; eauto.
-    * order_tac.
-    * exch 0. apply ImpLForAll_prev with (φ1 := φ1). exch 0. exact HPψ.
-- apply ImpLExists. eapply IHW; eauto.
-  + assert ( (ForAll (φ1 → φ2 〔 S' 〕)) ≺f  ((Exists φ1) → φ2) ).
-    unfold form_order.
-    simpl.
-    pose (weight_subst_S φ2) as H1.
-    simpl in H1.
-    rewrite H1.
-    lia.
-    order_tac.
-  + exch 0. apply ImpLExists_rev. exch 0. exact HPψ.
-Admitted.
+  apply IHHPφ2. lia.
+  exch 0. eapply ImpLImp_prev. exch 0. exact HPψ.
+- apply cut_principal_add with (w := w) (φ := (ForAll φ));
+    try easy; simpl in *; try lia.
+  right.
+  exists φ. easy.
+  apply ForAllR.
+  easy.
+- apply ForAllL with (t := t). eapply IHHPφ; eauto.
+  exch 0. exch 1. apply ForAllL_rev. exch 0. exact HPψ.
+- apply IHw with (φ := (subst_form (bind_var t) φ)).
+  rewrite weight_subst_f. 
+  lia.
+  easy.
+  apply ExistsL_rev_specialised.
+  easy.
+- apply ExistsL. apply IHHPφ. rewrite weight_subst_f. lia.
+  exch 0. backward_map. apply ExistsL_rev. exch 0. exact HPψ.
+- apply ImpLForAll.  assumption.
+  apply IHHPφ2. lia.
+  exch 0. apply ImpLForAll_prev with (φ1 := φ1). exch 0. easy.
+- apply ImpLExists. eapply IHHPφ; eauto.
+  exch 0. apply ImpLExists_rev. exch 0. exact HPψ.
+Qed.
 
 (* Multiplicative cut rule *)
 Theorem cut Γ Γ' φ ψ :
